DS: implemented first execution part of fake cert attacker

denning-sacco-central-auth/DS.Attacker.fst
@@ -18,37 +18,56 @@ module A = AttackerAPI
 
 val query_secret_key:
     idx_state:nat -> idx_corrupt:nat -> idx_query:nat ->
-    p:principal -> LCrypto (A.pub_bytes idx_query) (L.pki S.ds_preds)
-    (requires (fun t0 -> idx_state < idx_query /\ idx_corrupt < idx_query /\ idx_query <= trace_len t0 /\ was_corrupted_at idx_corrupt p 0 0))
-    (ensures (fun t0 _ t1 -> trace_len t1 == trace_len t0))
-let query_secret_key idx_state idx_corrupt idx_query p =
-    let t = A.query_state_i idx_state idx_corrupt idx_query p 0 0 in
-    match A.split t with
+    p:principal -> s:nat -> v:nat -> 
+    LCrypto (A.pub_bytes idx_query) (L.pki S.ds_preds)
+    (requires (fun t0 -> idx_state < idx_query /\ idx_corrupt < idx_query /\ idx_query <= trace_len t0 /\ was_corrupted_at idx_corrupt p s v))
+    (ensures (fun t0 _ t1 -> t1 == t0))
+let query_secret_key idx_state idx_corrupt idx_query p s v =
+    let t = A.query_state_i idx_state idx_corrupt idx_query p s v in
+    match A.split t with 
     | Success (tag, b) -> // tag == PKI
-      (match A.split b with
+      (match A.split b with 
       | Success (tag, b) -> b // Due to the string on key-usages in LabeledPKI, we need to split again
       | _ -> b)
-(*      (match split b with
-	| Success (tag', b) -> b // tag == SecretKey
-	| _ -> error "incorrect tag") *)
     | _ -> error "incorrect tag"
 
-let attacker_issue_fake_cert (#i:timestamp) (srv eve:principal)
-  (sk_srv pk_e pk_a: A.pub_bytes i) (msg1_idx:timestamp) :
+val query_public_key:
+    idx_state:nat -> idx_corrupt:nat -> idx_query:nat ->
+    p:principal -> s:nat -> v:nat -> 
+    LCrypto (A.pub_bytes idx_query) (L.pki S.ds_preds)
+    (requires (fun t0 -> idx_state < idx_query /\ idx_corrupt < idx_query /\ idx_query <= trace_len t0 /\ was_corrupted_at idx_corrupt p s v))
+    (ensures (fun t0 _ t1 -> t1 == t0))
+let query_public_key idx_state idx_corrupt idx_query p s v =
+    let t = A.query_state_i idx_state idx_corrupt idx_query p s v in
+    match A.split t with 
+    | Success (tag, b) -> // tag == PKI
+      (match A.split b with 
+      // Due to the string on key-usages in LabeledPKI, we need to split again
+      | Success (tag, b) -> (match A.split b with 
+			   | Success (tag, b) -> b // public key contains peer name
+			   | _ -> b) 
+      | _ -> b)
+    | _ -> error "incorrect tag"
+
+let attacker_issue_fake_cert (#i:timestamp) (eve:principal)
+  (sigk_srv pk_a pk_e: A.pub_bytes i) (msg1_idx:timestamp) :
   Crypto (msg2_idx:timestamp & c_out:clock)
   (requires (fun t0 -> msg1_idx < trace_len t0 /\
     later_than (trace_len t0) i))
   (ensures (fun t0 r t1 ->
     match r with
     | Success (|mi,c_out|) ->
-      A.attacker_modifies_trace t0 t1 /\
-      trace_len t1 == (trace_len t0) + 1 /\
+      (exists it. A.attacker_modifies_trace t0 it /\
+      A.attacker_modifies_trace it t1) /\
+      trace_len t1 == (trace_len t0) + 3 /\
       later_than (trace_len t1) (trace_len t0) /\
-      mi == trace_len t0 /\
+      mi == (trace_len t1) - 1 /\
       clock_get c_out == 1
-    | Error _ -> t0 == t1)) =
+    | Error _ -> t0 == t1 \/
+      (A.attacker_modifies_trace t0 t1 /\
+      later_than (trace_len t1) (trace_len t0)))) =
   // receive and parse first message
-  let (|t_m1,ser_msg1|) = A.receive_i msg1_idx srv in
+  let (|t_m1,ser_msg1|) = A.receive_i msg1_idx M.auth_srv in
 
   match
     A.split ser_msg1 `bind` (fun (tag_bytes, rest) ->
@@ -66,23 +85,28 @@ let attacker_issue_fake_cert (#i:timestamp) (srv eve:principal)
     let t = global_timestamp () in
     let c_new = clock_new () in
 
+    // generate sign nonce
+    let (|t_n_sig,n_sig|) = A.pub_rand_gen (nonce_usage "SIG_NONCE") in
+
     // create legitimate certificate for alice
-    let now = global_timestamp () in
-    let t_bytes = A.pub_bytes_later 0 now (A.nat_to_pub_bytes 0 t) in
-    let a_bytes = A.pub_bytes_later t_m1 now a_bytes in
-    let pk_a = A.pub_bytes_later i now pk_a in
-    let cert_a_tag = A.pub_bytes_later 0 now (A.string_to_pub_bytes "cert_a") in
+    let t_bytes = A.pub_bytes_later 0 t_n_sig (A.nat_to_pub_bytes 0 t) in
+    let a_bytes = A.pub_bytes_later t_m1 t_n_sig a_bytes in
+    let pk_a = A.pub_bytes_later i t_n_sig pk_a in
+    let cert_a_tag = A.pub_bytes_later 0 t_n_sig (A.string_to_pub_bytes "cert_a") in
     let ser_cert_a = A.concat cert_a_tag (A.concat a_bytes (A.concat pk_a t_bytes)) in
+    let sigk_srv = A.pub_bytes_later i t_n_sig sigk_srv in
+    let sig_cert_a = A.sign sigk_srv n_sig ser_cert_a in
 
     // create fake certificate for bob
-    let b_bytes = A.pub_bytes_later t_m1 now b_bytes in
-    let pk_e = A.pub_bytes_later i now pk_e in
-    let cert_b_tag = A.pub_bytes_later 0 now (A.string_to_pub_bytes "cert_b") in
+    let b_bytes = A.pub_bytes_later t_m1 t_n_sig b_bytes in
+    let pk_e = A.pub_bytes_later i t_n_sig pk_e in
+    let cert_b_tag = A.pub_bytes_later 0 t_n_sig (A.string_to_pub_bytes "cert_b") in
     let ser_fake_cert_b = A.concat cert_b_tag (A.concat b_bytes (A.concat pk_e t_bytes)) in
+    let sig_fake_cert_b = A.sign sigk_srv n_sig ser_fake_cert_b in
 
     // create and send second message
-    let msg2_tag = A.pub_bytes_later 0 now (A.string_to_pub_bytes "msg2") in
-    let ser_msg2 = A.concat msg2_tag (A.concat ser_cert_a ser_fake_cert_b) in
+    let msg2_tag = A.pub_bytes_later 0 t_n_sig (A.string_to_pub_bytes "msg2") in
+    let ser_msg2 = A.concat msg2_tag (A.concat sig_cert_a sig_fake_cert_b) in
 
-    att_send #now c_new srv a ser_msg2
+    att_send #t_n_sig c_new M.auth_srv a ser_msg2
   | Error e -> error e
