denning-sacco-central-auth/DS.Debug.fst
@@ -13,6 +13,7 @@ open SecurityLemmas
 open DS.Messages
 open DS.Sessions
 open DS.Protocol
+open DS.Attacker
 
 
 val benign_attacker:
@@ -46,6 +47,62 @@ let benign_attacker () =
   let (msg2_idx, srv_sess_idx, c_sm2) = server_send_msg_2 msg1_idx in
   let (msg3_idx, c_sm3) = initiator_send_msg_3 c_sm2 a msg2_idx a_sess_idx in
   let (b_sess_idx, c_end) = responder_recv_msg_3 c_sm3 b msg3_idx in
+  ()
+
+val fake_cert_attacker:
+  unit ->
+  LCrypto unit (pki ds_preds)
+  (requires fun _ -> True)
+  (ensures fun _ _ _ -> True)
+
+let fake_cert_attacker () =
+   let a:principal = "alice" in
+  let b:principal = "bob" in
+  let e:principal = "eve" in
+
+  let now = global_timestamp () in
+  let sigk_a_idx = gen_private_key #ds_preds #now a SIG "DS.sig_key" in
+  let now = global_timestamp () in
+  let sk_b_idx = gen_private_key #ds_preds #now b PKE "DS.pke_key" in
+  let before_sk_e = global_timestamp () in
+  let sk_e_idx = gen_private_key #ds_preds #before_sk_e e PKE "DS.pke_key" in
+  let before_sigk_srv = global_timestamp () in
+  let sigk_srv_idx = gen_private_key #ds_preds #before_sigk_srv auth_srv SIG "DS.sig_key" in
+
+  let before_pk_a = global_timestamp () in
+  let pk_a_srv_idx = install_public_key #ds_preds #before_pk_a a auth_srv SIG "DS.sig_key" in
+  let now = global_timestamp () in
+  let pk_b_srv_idx = install_public_key #ds_preds #now b auth_srv PKE "DS.pke_key" in
+  let before_pk_e = global_timestamp () in
+  let pk_e_srv_idx = install_public_key #ds_preds #before_pk_e e auth_srv PKE "DS.pke_key" in
+  let now = global_timestamp () in
+  let verk_srv_a_idx = install_public_key #ds_preds #now auth_srv a SIG "DS.sig_key" in
+  let now = global_timestamp () in
+  let verk_srv_b_idx = install_public_key #ds_preds #now auth_srv b SIG "DS.sig_key" in
+
+  // compromise eve's secret key
+  let idx_comp_e = compromise e sk_e_idx 0 in
+  let now = global_timestamp () in
+  let sk_e = query_secret_key (before_sk_e + 1) idx_comp_e now e sk_e_idx 0 in
+
+  // compromise server's secret key and pub keys of eve and alice
+  let idx_comp_srv = compromise auth_srv sigk_srv_idx 0 in
+  let after_comp_sigk_srv = global_timestamp () in
+  let sigk_srv = query_secret_key (before_sigk_srv + 1) idx_comp_srv after_comp_sigk_srv auth_srv sigk_srv_idx 0 in
+
+  let idx_comp_srv = compromise auth_srv pk_e_srv_idx 0 in
+  let after_comp_pk_e = global_timestamp () in
+  let pk_e = query_public_key (before_pk_e + 1) idx_comp_srv after_comp_pk_e auth_srv pk_e_srv_idx 0 in
+
+  let idx_comp_srv = compromise auth_srv pk_a_srv_idx 0 in
+  let after_comp_pk_a = global_timestamp () in
+  let pk_a = query_public_key (before_pk_a + 1) idx_comp_srv after_comp_pk_a auth_srv pk_a_srv_idx 0 in
+
+  let sigk_srv = pub_bytes_later after_comp_sigk_srv after_comp_pk_a sigk_srv in
+  let pk_e = pub_bytes_later after_comp_pk_e after_comp_pk_a pk_e in
+
+  let (msg1_idx, a_sess_idx) = initiator_send_msg_1 a b in
+  let (|msg2_idx,c_out|) = attacker_issue_fake_cert e sigk_srv pk_a pk_e msg1_idx in
   ()
 
 let benign () : LCrypto unit (pki ds_preds)
